First half of proof of trivial determinism

src/ReactorModel/Determinism/ExecutionStep.lean
@@ -2,95 +2,117 @@ import ReactorModel.Determinism.InstExecution
 
 namespace Execution
 
+open Classical 
 open State (Closed)
 
 variable [State.Nontrivial s] [State.Nontrivial s₁]
 
-theorem AdvanceTag.closed : (s₁ ⇓- s₂) → Closed s₁
+namespace AdvanceTag
+
+theorem closed : (s₁ ⇓- s₂) → Closed s₁
   | ⟨_, h⟩ => h
 
-theorem AdvanceTag.not_Closed : (s₁ ⇓- s₂) → ¬(Closed s₂)
+theorem not_Closed : (s₁ ⇓- s₂) → ¬(Closed s₂)
   | ⟨hg, _⟩, hc =>
     absurd (s₁.ctx.advanceTag_progress_empty $ s₁.tag_lt_nextTag hg) hc.progress_not_empty
 
-theorem AdvanceTag.nonrepeatable (a₁ : s₁ ⇓- s₂) (a₂ : s₂ ⇓- s₃) : False :=
+theorem nonrepeatable (a₁ : s₁ ⇓- s₂) (a₂ : s₂ ⇓- s₃) : False :=
   absurd a₂.closed a₁.not_Closed
 
-theorem AdvanceTag.tag_lt : (s₁ ⇓- s₂) → s₁.tag < s₂.tag
+theorem tag_lt : (s₁ ⇓- s₂) → s₁.tag < s₂.tag
   | mk .. => by simp [Context.advanceTag_strictly_increasing]
 
-theorem AdvanceTag.determinisic : (s ⇓- s₁) → (s ⇓- s₂) → s₁ = s₂
+theorem determinisic : (s ⇓- s₁) → (s ⇓- s₂) → s₁ = s₂
   | ⟨h₁, _⟩, ⟨h₂, _⟩ => by simp [Option.some_inj.mp $ h₂ ▸ h₁]
 
-instance AdvanceTag.preserves_Nontrivial [State.Nontrivial s₁] {e : s₁ ⇓- s₂} : 
-    State.Nontrivial s₂ :=
+instance preserves_Nontrivial [State.Nontrivial s₁] {e : s₁ ⇓- s₂} : State.Nontrivial s₂ :=
   match e with | ⟨_, _⟩ => inferInstance
 
-theorem ClosedExecution.not_Closed (e : s₁ ⇓| s₂) : ¬(Closed s₁) := 
-  State.Open.not_Closed e.open
+theorem rtr_eq : (s₁ ⇓- s₂) → s₁.rtr = s₂.rtr
+  | ⟨_, _⟩ => rfl
 
-theorem ClosedExecution.tag_eq (e : s₁ ⇓| s₂) : s₁.tag = s₂.tag :=
+end AdvanceTag
+
+namespace ClosedExecution
+
+theorem not_Closed (e : s₁ ⇓| s₂) : ¬(Closed s₁) := by
+  simp [Closed]
+  exact e.fresh ▸ State.Nontrivial.nontrivial.symm 
+
+theorem tag_eq (e : s₁ ⇓| s₂) : s₁.tag = s₂.tag :=
   e.exec.tag_eq
 
-theorem ClosedExecution.preserves_rcns (e : s₁ ⇓| s₂) : s₁.rtr.ids .rcn = s₂.rtr.ids .rcn := by
+theorem preserves_rcns (e : s₁ ⇓| s₂) : s₁.rtr.ids .rcn = s₂.rtr.ids .rcn := by
   simp [Finset.ext_iff, Reactor.ids_mem_iff_obj?, e.exec.preserves_rcns]
 
-theorem ClosedExecution.rcns_eq (e₁ : s ⇓| s₁) (e₂ : s ⇓| s₂) : s₁.rtr.ids .rcn = s₂.rtr.ids .rcn :=
+theorem rcns_eq (e₁ : s ⇓| s₁) (e₂ : s ⇓| s₂) : s₁.rtr.ids .rcn = s₂.rtr.ids .rcn :=
   e₁.preserves_rcns ▸ e₂.preserves_rcns
   
-theorem ClosedExecution.rcns_Nodup (e : s₁ ⇓| s₂) : e.rcns.Nodup := 
+theorem rcns_Nodup (e : s₁ ⇓| s₂) : e.rcns.Nodup := 
   e.exec.rcns_nodup
 
-theorem ClosedExecution.progress_def (e : s₁ ⇓| s₂) : s₂.progress = s₁.rtr.ids .rcn :=
+theorem progress_def (e : s₁ ⇓| s₂) : s₂.progress = s₁.rtr.ids .rcn :=
   e.preserves_rcns ▸ e.closed
 
-theorem ClosedExecution.mem_rcns_iff (e : s₁ ⇓| s₂) (rcn : ID) : 
-    rcn ∈ e.rcns ↔ (rcn ∈ s₁.rtr.ids .rcn ∧ rcn ∉ s₁.progress) :=
+theorem mem_rcns_iff (e : s₁ ⇓| s₂) : rcn ∈ e.rcns ↔ (rcn ∈ s₁.rtr.ids .rcn ∧ rcn ∉ s₁.progress) :=
   e.progress_def ▸ e.exec.mem_rcns_iff rcn
 
-theorem ClosedExecution.rcns_perm (e₁ : s ⇓| s₁) (e₂ : s ⇓| s₂) : e₁.rcns ~ e₂.rcns := by
+theorem rcns_perm (e₁ : s ⇓| s₁) (e₂ : s ⇓| s₂) : e₁.rcns ~ e₂.rcns := by
   simp [List.perm_ext e₁.rcns_Nodup e₂.rcns_Nodup, e₁.mem_rcns_iff, e₂.mem_rcns_iff]
 
-theorem ClosedExecution.ctx_eq (e₁ : s ⇓| s₁) (e₂ : s ⇓| s₂) : s₁.ctx = s₂.ctx :=
+theorem ctx_eq (e₁ : s ⇓| s₁) (e₂ : s ⇓| s₂) : s₁.ctx = s₂.ctx :=
   e₁.exec.ctx_eq ▸ e₂.exec.ctx_eq ▸ (Context.process_perm_eq $ e₁.rcns_perm e₂)
 
-theorem ClosedExecution.deterministic (e₁ : s ⇓| s₁) (e₂ : s ⇓| s₂) : s₁ = s₂ :=
+theorem deterministic (e₁ : s ⇓| s₁) (e₂ : s ⇓| s₂) : s₁ = s₂ :=
   e₁.exec.deterministic e₂.exec $ e₁.ctx_eq e₂
 
-theorem ClosedExecution.step_determined (e : s ⇓| s₁) (a : s ⇓- s₂) : False :=
+theorem step_determined (e : s ⇓| s₁) (a : s ⇓- s₂) : False :=
   absurd a.closed e.not_Closed
 
-instance ClosedExecution.preserves_Nontrivial [h : State.Nontrivial s₁] {e : s₁ ⇓| s₂} : 
-    State.Nontrivial s₂ where
+instance preserves_Nontrivial [h : State.Nontrivial s₁] {e : s₁ ⇓| s₂} : State.Nontrivial s₂ where
   nontrivial := e.preserves_rcns ▸ h.nontrivial
 
-theorem ClosedExecution.nonrepeatable (e₁ : s₁ ⇓| s₂) (e₂ : s₂ ⇓| s₃) : False :=
+theorem nonrepeatable (e₁ : s₁ ⇓| s₂) (e₂ : s₂ ⇓| s₃) : False :=
   have := e₁.preserves_Nontrivial -- TODO: Make this work via type class inference.
   absurd e₁.closed $ e₂.not_Closed
 
-theorem ClosedExecution.progress_ssubset (e : s₁ ⇓| s₂) : s₁.progress ⊂ s₂.progress := by
+theorem progress_ssubset (e : s₁ ⇓| s₂) : s₁.progress ⊂ s₂.progress := by
   have := e.preserves_Nontrivial -- TODO: Make this work via type class inference.
-  rw [e.open]
+  rw [e.fresh]
   exact Finset.nonempty.empty_ssubset $ e.closed.progress_not_empty
 
-instance Step.preserves_Nontrivial [State.Nontrivial s₁] {e : s₁ ⇓ s₂} : State.Nontrivial s₂ :=
-  match e with 
-  | close e => e.preserves_Nontrivial
-  | advance a => a.preserves_Nontrivial
+theorem trivial_rtr_eq [State.Trivial s₁] (e : s₁ ⇓| s₂) : s₁.rtr = s₂.rtr :=
+  e.exec.trivial_rtr_eq
 
-theorem Step.tag_le : (s₁ ⇓ s₂) → s₁.tag ≤ s₂.tag
+end ClosedExecution
+
+namespace Step
+
+theorem tag_le : (s₁ ⇓ s₂) → s₁.tag ≤ s₂.tag
   | close e   => le_of_eq e.tag_eq
   | advance a => le_of_lt a.tag_lt
 
-protected theorem Step.deterministic : (s ⇓ s₁) → (s ⇓ s₂) → s₁ = s₂
+theorem deterministic : (s ⇓ s₁) → (s ⇓ s₂) → s₁ = s₂
   | close e₁, close e₂                      => e₁.deterministic e₂
   | advance a₁, advance a₂                  => a₁.determinisic a₂
   | close e, advance a | advance a, close e => e.step_determined a |>.elim
 
-theorem Step.seq_tag_lt : (s₁ ⇓ s₂) → (s₂ ⇓ s₃) → s₁.tag < s₃.tag
-  | advance a₁, advance a₂ => a₁.nonrepeatable a₂ |>.elim
+theorem seq_tag_lt : (s₁ ⇓ s₂) → (s₂ ⇓ s₃) → s₁.tag < s₃.tag
   | close e₁,   close e₂   => e₁.nonrepeatable e₂ |>.elim
-  | advance a,  close e    => e.tag_eq ▸ a.tag_lt
+  | advance a₁, advance a₂ => a₁.nonrepeatable a₂ |>.elim
   | close e,    advance a  => e.tag_eq ▸ a.tag_lt
+  | advance a,  close e    => e.tag_eq ▸ a.tag_lt
+
+theorem trivial_rtr_eq [State.Trivial s₁] : (s₁ ⇓ s₂) → s₁.rtr = s₂.rtr
+  | close e => e.trivial_rtr_eq 
+  | advance a => a.rtr_eq
+
+instance preserves_Nontrivial [State.Nontrivial s₁] : (s₁ ⇓ s₂) → State.Nontrivial s₂
+  | close e => e.preserves_Nontrivial
+  | advance a => a.preserves_Nontrivial
+
+instance preserves_Trivial [State.Trivial s₁] : (s₁ ⇓ s₂) → State.Trivial s₂ := sorry
+
+end Step
 
 end Execution
