src/ReactorModel/Determinism/Execution.lean
@@ -1,19 +1,36 @@
 import ReactorModel.Determinism.ExecutionStep
 
 open Classical 
-open Execution (State)
 
-theorem Execution.tag_le : (s₁ ⇓* s₂) → s₁.tag ≤ s₂.tag
-  | refl => by simp
+namespace Execution
+
+theorem trivial_rtr_eq [State.Trivial s₁] : (s₁ ⇓* s₂) → s₁.rtr = s₂.rtr
+  | refl      => rfl
+  | step e e' => 
+    have := e.preserves_Trivial -- TODO: Make this work via type class inference.
+    e.trivial_rtr_eq ▸ e'.trivial_rtr_eq
+
+theorem trivial_ctx_eq [State.Trivial s₁] : (s₁ ⇓* s₂) →
+  s₂.ctx = (s₁.ctx.mark $ s₁.rtr.scheduledTags.filter fun g => s₁.tag < g ∧ g ≤ s₂.tag) :=
+    sorry
+
+theorem trivial_deterministic [trivial : State.Trivial s] 
+    (e₁ : s ⇓* s₁) (e₂ : s ⇓* s₂) (ht : s₁.tag = s₂.tag) : s₁ = s₂ := by
+  ext1
+  · exact e₁.trivial_rtr_eq ▸ e₂.trivial_rtr_eq 
+  · rw [e₁.trivial_ctx_eq, e₂.trivial_ctx_eq, ht]
+
+theorem tag_le : (s₁ ⇓* s₂) → s₁.tag ≤ s₂.tag
+  | refl      => le_refl _
   | step e e' => le_trans e.tag_le e'.tag_le
 
-theorem Execution.seq_progress_ssubset_or_tag_lt [State.Nontrivial s₁] : 
+theorem seq_progress_ssubset_or_tag_lt [State.Nontrivial s₁] : 
     (s₁ ⇓ s₂) → (s₂ ⇓* s₃) → (s₁.progress ⊂ s₃.progress) ∨ (s₁.tag < s₃.tag)
   | e₁₂,        .step e e' => .inr $ lt_of_lt_of_le (e₁₂.seq_tag_lt e) e'.tag_le
   | .close e,   .refl      => .inl $ e.progress_ssubset
   | .advance a, .refl      => .inr $ a.tag_lt
 
-theorem Execution.nontrivial_deterministic [State.Nontrivial s] :
+theorem nontrivial_deterministic [State.Nontrivial s] :
     (s ⇓* s₁) → (s ⇓* s₂) → (s₁.tag = s₂.tag) → (s₁.progress = s₂.progress) → s₁ = s₂
   | refl, refl, _, _ => rfl
   | step e₁ e₁', step e₂ e₂', ht, hp => 
@@ -24,10 +41,10 @@ theorem Execution.nontrivial_deterministic [State.Nontrivial s] :
     | .inl h => absurd hp $ Finset.ssubset_ne (by simp_all) 
     | .inr h => absurd ht $ ne_of_lt h
 
-protected theorem Execution.deterministic : 
-    (s ⇓* s₁) → (s ⇓* s₂) → (s₁.tag = s₂.tag) → (s₁.progress = s₂.progress) → s₁ = s₂ := by
-  by_cases State.Nontrivial s
-  case pos => exact nontrivial_deterministic
-  case neg =>
-    sorry
+theorem deterministic : 
+    (s ⇓* s₁) → (s ⇓* s₂) → (s₁.tag = s₂.tag) → (s₁.progress = s₂.progress) → s₁ = s₂ := 
+  if h : State.Nontrivial s 
+  then nontrivial_deterministic
+  else fun e₁ e₂ ht _ => trivial_deterministic e₁ e₂ ht (trivial := ⟨h⟩)
   
+end Execution
